ott/coq/AilTypingStatements_defns.v
@@ -1,0 +1,107 @@
+Require Import Common.
+Require Import Implementation.
+Require Import AilTypes.
+Require Import AilSyntax.
+
+Require Import AilTypesAux_defns.
+Require Import AilWf_defns.
+Require Import AilTyping_defns.
+Require Import Context_defns.
+
+Inductive wellFormedBinding : identifier * (qualifiers * ctype) -> Prop :=
+ | WellFormedBinding v q t :
+     wfLvalue q t ->
+     wellFormedBinding (v, (q, t)).
+
+Inductive wellFormedBindings : bindings -> Prop :=
+ | WellFormedBindings bs :
+     disjointBindings bs ->
+     allList wellFormedBinding bs ->
+     wellFormedBindings bs.
+
+Inductive wellTypedDefinition {A B} P G (S : sigma  A B) : identifier * expression B -> Prop :=
+  | WellTypedDefinition :
+      forall v e q t,
+        lookup G v (q, t) ->
+        assignable P G S t e ->
+        wellTypedDefinition P G S (v, e).
+
+Inductive wellTypedStatement' {A B} P G (S : sigma A B) : ctype -> statement' A B -> Prop :=    (* defn wellTypedStatement *)
+ | WellTypedStatement'_Label : forall t_return l s,
+     wellTypedStatement  P G S t_return s ->
+     wellTypedStatement' P G S t_return (Label l s)
+ | WellTypedStatement'_Case : forall t_return ic it s,
+     typeOfConstant P ic it ->
+     wellTypedStatement  P G S t_return s ->
+     wellTypedStatement' P G S t_return (Case ic s)
+ | WellTypedStatement'_Default : forall t_return s,
+     wellTypedStatement  P G S t_return s ->
+     wellTypedStatement' P G S t_return (Default s)
+ | WellTypedStatement'_Block : forall t_return bs ss,
+     wellFormedBindings bs ->
+     freshBindings bs S ->
+     allList (wellTypedStatement P (Context.add_bindings bs G) S t_return) ss ->
+     wellTypedStatement' P G S t_return (Block bs ss)
+ | WellTypedStatement'_Skip : forall t_return,
+     wellTypedStatement' P G S t_return Skip
+ | WellTypedStatement'_Expression : forall t_return e,
+     typeable P G S e ->
+     wellTypedStatement' P G S t_return (Expression e)
+ | WellTypedStatement'_If : forall t_return e s1 s2 t,
+     typeOfRValue P G S e t ->
+     scalar t ->
+     wellTypedStatement  P G S t_return s1 ->
+     wellTypedStatement  P G S t_return s2 ->
+     wellTypedStatement' P G S t_return (If e s1 s2)
+ | WellTypedStatement'_Switch : forall t_return e s t,
+     typeOfRValue P G S e t ->
+     integer t ->
+     wellTypedStatement  P G S t_return s ->
+     wellTypedStatement' P G S t_return (Switch e s)
+ | WellTypedStatement'_While : forall t_return e s t,
+     typeOfRValue P G S e t ->
+     scalar t ->
+     wellTypedStatement  P G S t_return s ->
+     wellTypedStatement' P G S t_return (While e s)
+ | WellTypedStatement'_Do : forall t_return s e t,
+     typeOfRValue P G S e t ->
+     scalar t ->
+     wellTypedStatement  P G S t_return s ->
+     wellTypedStatement' P G S t_return (Do s e)
+ | WellTypedStatement'_Goto : forall t_return l,
+     wellTypedStatement' P G S t_return (Goto l)
+ | WellTypedStatement'_Continue : forall t_return,
+     wellTypedStatement' P G S t_return Continue
+ | WellTypedStatement'_Break : forall t_return,
+     wellTypedStatement' P G S t_return Break
+ | WellTypedStatement'_ReturnVoid :
+     wellTypedStatement' P G S Void ReturnVoid
+ | WellTypedStatement'_Return : forall t_return e,
+     assignable P G S t_return e ->
+     wellTypedStatement' P G S t_return (Return e)
+ | WellTypedStatement'_Declaration : forall t_return ds,
+     allList (wellTypedDefinition P G S) ds ->
+     wellTypedStatement' P G S t_return (Declaration ds)
+with wellTypedStatement {A B} P G (S : sigma A B) : ctype -> statement A B -> Prop :=
+ | WellTypedStatement_AnnotatedStatement : forall t_return a s,
+     wellTypedStatement' P G S t_return s ->
+     wellTypedStatement  P G S t_return (AnnotatedStatement a s).
+
+Inductive wellTypedFunction {A B} P (S : sigma A B) : (ctype * bindings) * statement A B -> Prop :=
+  | WellTypedFunction t_return bs s :
+      wellFormedBindings bs ->
+      freshBindings bs S ->
+      wfType (Function t_return (parameters_of_bindings bs)) ->
+      wellTypedStatement P (Context.add_bindings bs nil) S t_return s ->
+      wellTypedFunction P S (t_return, bs, s).      
+
+Inductive wellTypedSigma {A B} P (S : sigma A B) : Prop :=
+ | WellTypedSigma :
+     (forall v p, lookup S v p -> wellTypedFunction P S p) ->
+     wellTypedSigma P S.
+
+Inductive wellTypedProgram {A B} P : program A B -> Prop :=    (* defn wellTypedProgram *)
+ | WellTypedProgram main S s:
+       lookup S main (Basic (Integer (Signed Int)), nil, s) ->
+       wellTypedSigma P S ->
+       wellTypedProgram P (main, S).
